generic/Zeta.Generic.TSLog.fsti
@@ -4,6 +4,7 @@ open FStar.Seq
 open Zeta.SeqAux
 open Zeta.Interleave
 open Zeta.Time
+open Zeta.IdxFn
 open Zeta.GenericVerifier
 open Zeta.Generic.Thread
 open Zeta.Generic.Global
@@ -11,6 +12,7 @@ open Zeta.Generic.Interleave
 
 module I = Zeta.Interleave
 module G = Zeta.Generic.Global
+module T = Zeta.Generic.Thread
 module S = FStar.Seq
 module SA = Zeta.SeqAux
 
@@ -24,3 +26,12 @@ val lemma_prefix_clock_sorted (#vspec #n:_) (itsl: its_log vspec n) (i:nat{i <= 
         [SMTPat (prefix itsl i)]
 
 val create (#vspec:_) (gl: G.verifiable_log vspec): (itsl:its_log vspec (S.length gl){to_glog itsl == gl})
+
+val prefix_within_epoch (#vspec #n:_) (ep: epoch) (itsl: its_log vspec n)
+  : itsl': its_log vspec n {itsl' `prefix_of` itsl}
+
+val lemma_appfn_calls_within_epoch (#vspec #n:_) (ep: epoch) (itsl: its_log vspec n)
+  : Lemma (ensures (let itsl_ep = prefix_within_epoch ep itsl in
+                    let gl_ep = to_glog itsl_ep in
+                    let gl = to_glog itsl in
+                    G.appfn_calls gl_ep = G.appfn_calls_within_ep ep gl))
