high2/Zeta.High.Correctness.fst
@@ -1,5 +1,43 @@
 module Zeta.High.Correctness
 
+open Zeta.App
+open Zeta.Time
+open Zeta.AppSimulate
 open Zeta.High.Verifier
+open Zeta.Generic.Global
+open Zeta.Generic.Interleave
+open Zeta.Generic.TSLog
+open Zeta.High.Global
+open Zeta.High.Interleave
+open Zeta.HashCollision
 
+module I = Zeta.Interleave
 module G = Zeta.Generic.Global
+module HG = Zeta.High.Global
+
+let lemma_verifier_correct
+  (#app:_)
+  (epmax: epoch)
+  (gl: HG.ms_verifiable_log app epmax{~ (seq_consistent (appfn_calls_within_ep epmax gl))})
+  : hash_collision app
+  = (* sequence of sequence of app fn calls and results *)
+    let app_calls_ss = appfn_calls_within_ep epmax gl in
+
+    (* interleaving of gl ordered by time of each log entry *)
+    let itsl = create gl in
+
+    (* prefix upto epoch epmax *)
+    let itsl_ep = prefix_within_epoch epmax itsl in
+    lemma_appfn_calls_within_epoch epmax itsl;
+    assert(G.appfn_calls (to_glog itsl_ep) = app_calls_ss);
+
+    if is_eac itsl_ep then (
+      (* is_eac itsl_ep ==> this sequence is sequentially consistent *)
+      lemma_eac_implies_appfn_calls_seq_consistent itsl_ep;
+      assert(seq_consistent (G.appfn_calls (to_glog itsl_ep)));
+
+      hash_collision_contra app
+    )
+    else
+
+    admit()
