utils/Zeta.MultiSet.SSeq.fst
@@ -4,3 +4,7 @@ let sseq2mset (#a:eqtype) (#f:cmp a) (s:sseq a) : mset a f
   = let open Zeta.Interleave in
     let il = some_interleaving s in
     seq2mset (i_seq il)
+
+let lemma_interleaving_multiset (#a:_) (#f:cmp a) (#n:_) (il: interleaving a n)
+  : Lemma (ensures (seq2mset #_ #f (i_seq il) == sseq2mset (s_seq il)))
+  = admit()
