generic/Zeta.HashCollision.fsti
@@ -9,3 +9,7 @@ open Zeta.Record
 type hash_collision (app: app_params) =
   | Collision: v1: value app ->
                v2: value app {v1 <> v2 /\ hashfn v1 = hashfn v2} -> hash_collision app
+
+let hash_collision_contra (app:app_params{False})
+  : hash_collision app
+  = Collision (AppV Null) (AppV Null)
