high2/Zeta.High.TSLog.fsti
@@ -1,0 +1,15 @@
+module Zeta.High.TSLog
+
+open Zeta.App
+open Zeta.Time
+open Zeta.Generic.TSLog
+open Zeta.High.Verifier
+open Zeta.High.Interleave
+
+module T = Zeta.Generic.TSLog
+
+let its_log (app: app_params)
+  = T.its_log (high_verifier_spec app)
+
+let neac_before_epoch (app n:_) (ep: epoch)
+  = itsl: its_log app n {not (is_eac (prefix_within_epoch ep itsl))}
