high2/Zeta.High.Verifier.EAC.fsti
@@ -1,0 +1,13 @@
+module Zeta.High.Verifier.EAC
+
+open Zeta.Time
+open Zeta.EAC
+open Zeta.High.Verifier
+open Zeta.High.TSLog
+
+(*
+val lemma_neac_implies_hash_collision
+  (#app:_)
+  (epmax: epoch)
+  (itsl: neac_before_epoch epmax )
+*)
