utils/Zeta.MultiSet.SSeq.fsti
@@ -5,7 +5,11 @@ module Zeta.MultiSet.SSeq
 
 open Zeta.SSeq
 open Zeta.MultiSet
+open Zeta.Interleave
 
 /// Construct a multiset from a seq of sequences
 
 val sseq2mset (#a:eqtype) (#f:cmp a) (s:sseq a) : mset a f
+
+val lemma_interleaving_multiset (#a:_) (#f:cmp a) (#n:_) (il: interleaving a n)
+  : Lemma (ensures (seq2mset #_ #f (i_seq il) == sseq2mset (s_seq il)))
